cedar-lean/Cedar/Validation/RequestEntityValidator.lean
@@ -102,30 +102,30 @@ For every entity in the store,
 For every action in the entity store, the action's ancestors are consistent
 with the ancestor information in the action store.
 -/
-def instanceOfSchema (entities : Entities) (ets : EntitySchema) (as : ActionSchema) : EntityValidationResult :=
+def instanceOfSchema (entities : Entities) (env : Environment) : EntityValidationResult :=
   do
     entities.toList.forM λ (uid, data) => instanceOfEntityData uid data
-    as.toList.forM λ (uid, data) => instanceOfActionSchemaData uid data
+    env.acts.toList.forM λ (uid, data) => instanceOfActionSchemaData uid data
 where
   instanceOfEntityTags (data : EntityData) (entry : EntitySchemaEntry) : Bool :=
     match entry.tags? with
-    | .some tty => data.tags.values.all (instanceOfType · tty ets)
+    | .some tty => data.tags.values.all (instanceOfType · tty env.ets)
     | .none     => data.tags == Map.empty
   instanceOfEntityData uid data :=
-    match ets.find? uid.ty with
+    match env.ets.find? uid.ty with
     |  .some entry =>
       if entry.isValidEntityEID uid.eid then
-        if instanceOfType data.attrs (.record entry.attrs) ets then
+        if instanceOfType data.attrs (.record entry.attrs) env.ets then
           if data.ancestors.all (λ ancestor =>
             entry.ancestors.contains ancestor.ty &&
-            instanceOfEntityType ancestor ancestor.ty ets.entityTypeMembers?) then
+            instanceOfEntityType ancestor ancestor.ty env.ets.entityTypeMembers?) then
             if instanceOfEntityTags data entry then .ok ()
             else .error (.typeError s!"entity tags inconsistent with type store")
           else .error (.typeError s!"entity ancestors inconsistent with type store")
         else .error (.typeError "entity attributes do not match type store")
       else .error (.typeError s!"invalid entity uid: {uid}")
     | _ =>
-      match as.find? uid with
+      match env.acts.find? uid with
       | .some _ =>
         if data.attrs == Map.empty then
           if data.tags == Map.empty then .ok ()
@@ -147,7 +147,7 @@ def validateRequest (schema : Schema) (request : Request) : RequestValidationRes
   else .error (.typeError "request could not be validated in any environment")
 
 def entitiesMatchEnvironment (env : Environment) (entities : Entities) : EntityValidationResult :=
-  instanceOfSchema entities env.ets env.acts
+  instanceOfSchema entities env
 
 def actionSchemaEntryToEntityData (ase : ActionSchemaEntry) : EntityData := {
   ancestors := ase.ancestors,
